Update FreeRTOS_tasks_noasserts_proofs_clz.v

timing/examples/FreeRTOS_tasks_noasserts_proofs_clz.v
@@ -45,7 +45,7 @@ Definition uxTopReadyPriority (gp : N) (mem : addr -> N) : N :=
     mem Ⓓ[gp ⊖ 1920].
 
 Definition addr_pxReadyTasksLists (gp : N) : N :=
-    gp - 924.
+    gp ⊖ 924.
 
 Definition vTaskSwitchContext_exit (t:trace) :=
   match t with (Addr a,_)::_ => match a with
@@ -53,6 +53,7 @@ Definition vTaskSwitchContext_exit (t:trace) :=
   | _ => false
   end | _ => false end.
 
+(* TODO : Rewrite postconditions, the if conditions are garbage from earlier versions *)
 Definition timing_postcondition (t : trace) (gp : N) (mem : addr -> N) : Prop :=
     if (uxSchedulerSuspended gp mem) =? 0 then
         cycle_count_of_trace t = 25 + 3 * time_branch + 17 * time_mem
@@ -131,11 +132,36 @@ Definition static_buffer_lengths_in_bytes (a : addr) : option N :=
 
 Definition smem_well_formed (gp : N) : Prop :=
     forall x y len_x len_y,
+                x <> y ->
                 static_buffer_lengths_in_bytes x = Some len_x ->
                 static_buffer_lengths_in_bytes y = Some len_y ->
             ~ overlap 32
                 (gp ⊖ x) len_x
                 (gp ⊖ y) len_y.
+
+Definition pxCurrentTCB_noverlap_static (gp : N) mem : Prop :=
+    forall x len_x,
+        static_buffer_lengths_in_bytes x = Some len_x ->
+        ~ overlap 32
+            (48 + pxCurrentTCB gp mem) 4
+            (gp ⊖ x) len_x.
+
+Definition pxCurrentTCB_noverlap_stackframe (gp base_sp : N) mem : Prop :=
+    ~ overlap 32
+        (48 + pxCurrentTCB gp mem) 4
+        (base_sp ⊖ 16) 16.
+
+Definition mem_pxCurrentTCB_noverlap_stackframe (gp base_sp : N) mem : Prop :=
+    ~ overlap 32
+        (mem Ⓓ[48 + pxCurrentTCB gp mem]) 4
+        (base_sp ⊖ 16) 16.
+
+Definition mem_pxCurrentTCB_noverlap_static (gp : N) mem : Prop :=
+    forall x len_x,
+        static_buffer_lengths_in_bytes x = Some len_x ->
+        ~ overlap 32
+            (mem Ⓓ[48 + pxCurrentTCB gp mem]) 4
+            (gp ⊖ x) len_x.
 
 Definition vTaskSwitchContext_timing_invs (_ : store) (p : addr) (base_sp : N) (t:trace) :=
 match t with (Addr a, s) :: t' => match a with
@@ -151,56 +177,85 @@ match t with (Addr a, s) :: t' => match a with
             /\ s R_A4 = Ⓓ(uxSchedulerSuspended gp mem) /\
             gp_sp_noverlap gp base_sp /\
             smem_well_formed gp /\
+            pxCurrentTCB_noverlap_static gp mem /\
+            pxCurrentTCB_noverlap_stackframe gp base_sp mem /\
+            mem_pxCurrentTCB_noverlap_stackframe gp base_sp mem /\
+            mem_pxCurrentTCB_noverlap_static gp mem /\
         cycle_count_of_trace t' = time_mem)
-    | 0x800013b4 => Some (exists mem gp, s V_MEM32 = Ⓜmem /\ s R_GP = Ⓓgp /\ s R_SP = Ⓓ(base_sp ⊖ 16) /\
+    | 0x800013b4 => Some (exists mem gp, s V_MEM32 = Ⓜmem /\ 
+        s R_GP = Ⓓgp /\ s R_SP = Ⓓ(base_sp ⊖ 16) /\
         s R_A5 = Ⓓ(mem Ⓓ[48 + pxCurrentTCB gp mem]) /\
         s R_A2 = Ⓓ(mem Ⓓ[mem Ⓓ[48 + pxCurrentTCB gp mem]]) /\
         s R_A4 = Ⓓ((0xa5a5a << 12) + 1445) /\
         gp_sp_noverlap gp base_sp /\
         smem_well_formed gp /\
+        pxCurrentTCB_noverlap_static gp mem /\
+        pxCurrentTCB_noverlap_stackframe gp base_sp mem /\
+        mem_pxCurrentTCB_noverlap_stackframe gp base_sp mem /\
+        mem_pxCurrentTCB_noverlap_static gp mem /\
         (uxSchedulerSuspended gp mem =? 0) = true /\
         cycle_count_of_trace t' = 6 + 7 * time_mem + time_branch)
-    | 0x800013bc => Some (exists mem gp, s V_MEM32 = Ⓜmem /\ s R_GP = Ⓓgp /\
+    | 0x800013bc => Some (exists mem gp, s V_MEM32 = Ⓜmem /\ 
+        s R_GP = Ⓓgp /\ s R_SP = Ⓓ(base_sp ⊖ 16) /\
         s R_A2 = Ⓓ(mem Ⓓ[mem Ⓓ[48 + pxCurrentTCB gp mem]]) /\
         s R_A3 = Ⓓ(mem Ⓓ[4 + mem Ⓓ[48 + pxCurrentTCB gp mem]]) /\
         s R_A5 = Ⓓ(mem Ⓓ[48 + pxCurrentTCB gp mem]) /\
         gp_sp_noverlap gp base_sp /\
         smem_well_formed gp /\
+        pxCurrentTCB_noverlap_static gp mem /\
+        pxCurrentTCB_noverlap_stackframe gp base_sp mem /\
+        mem_pxCurrentTCB_noverlap_stackframe gp base_sp mem /\
+        mem_pxCurrentTCB_noverlap_static gp mem /\
         (uxSchedulerSuspended gp mem =? 0) = true /\
         (mem Ⓓ[ mem Ⓓ[ 48 + pxCurrentTCB gp mem ] ] =? 0xa5a5a5a5) = true /\
         cycle_count_of_trace t' = 9 + 8 * time_mem + time_branch)
-    | 0x800013c4 => Some (exists mem gp, s V_MEM32 = Ⓜmem /\ s R_GP = Ⓓgp /\
+    | 0x800013c4 => Some (exists mem gp, s V_MEM32 = Ⓜmem /\ 
+        s R_GP = Ⓓgp /\ s R_SP = Ⓓ(base_sp ⊖ 16) /\
         s R_A3 = Ⓓ(mem Ⓓ[4 + mem Ⓓ[48 + pxCurrentTCB gp mem]]) /\
         s R_A4 = Ⓓ(mem Ⓓ[8 + mem Ⓓ[48 + pxCurrentTCB gp mem]]) /\
+        s R_A5 = Ⓓ(mem Ⓓ[48 + pxCurrentTCB gp mem]) /\
         gp_sp_noverlap gp base_sp /\
         smem_well_formed gp /\
-        s R_A5 = Ⓓ(mem Ⓓ[48 + pxCurrentTCB gp mem]) /\
+        pxCurrentTCB_noverlap_static gp mem /\
+        pxCurrentTCB_noverlap_stackframe gp base_sp mem /\
+        mem_pxCurrentTCB_noverlap_stackframe gp base_sp mem /\
+        mem_pxCurrentTCB_noverlap_static gp mem /\
         (mem Ⓓ[ mem Ⓓ[ 48 + pxCurrentTCB gp mem ] ] =? 0xa5a5a5a5) = true /\
         (mem Ⓓ[4 + mem Ⓓ[48 + pxCurrentTCB gp mem]] =? mem Ⓓ[mem Ⓓ[48 + pxCurrentTCB gp mem]]) = true /\
         (uxSchedulerSuspended gp mem =? 0) = true /\
         cycle_count_of_trace t' = 12 + 9 * time_mem + time_branch
     )
-    | 0x800013cc => Some (exists mem gp, s V_MEM32 = Ⓜmem /\ s R_GP = Ⓓgp /\
+    | 0x800013cc => Some (exists mem gp, s V_MEM32 = Ⓜmem /\ 
+        s R_GP = Ⓓgp /\ s R_SP = Ⓓ(base_sp ⊖ 16) /\
         s R_A3 = Ⓓ(mem Ⓓ[4 + mem Ⓓ[48 + pxCurrentTCB gp mem]]) /\
         s R_A4 = Ⓓ(mem Ⓓ[8 + mem Ⓓ[48 + pxCurrentTCB gp mem]]) /\
         s R_A5 = Ⓓ(mem Ⓓ[12 + mem Ⓓ[48 + pxCurrentTCB gp mem]]) /\
         gp_sp_noverlap gp base_sp /\
         smem_well_formed gp /\
+        pxCurrentTCB_noverlap_static gp mem /\
+        pxCurrentTCB_noverlap_stackframe gp base_sp mem /\
+        mem_pxCurrentTCB_noverlap_stackframe gp base_sp mem /\
+        mem_pxCurrentTCB_noverlap_static gp mem /\
         (mem Ⓓ[ mem Ⓓ[ 48 + pxCurrentTCB gp mem ] ] =? 0xa5a5a5a5) = true /\
         (mem Ⓓ[4 + mem Ⓓ[48 + pxCurrentTCB gp mem]] =? mem Ⓓ[mem Ⓓ[48 + pxCurrentTCB gp mem]]) = true /\
         (mem Ⓓ[8 + mem Ⓓ[48 + pxCurrentTCB gp mem]] =? mem Ⓓ[4 + mem Ⓓ[48 + pxCurrentTCB gp mem]]) = true /\
         (uxSchedulerSuspended gp mem =? 0) = true /\
         cycle_count_of_trace t' = 15 + 10 * time_mem + time_branch
     )
-    | 0x80001418 => Some (exists mem gp, s V_MEM32 = Ⓜmem /\ s R_GP = Ⓓgp /\
-        s R_A1 = Ⓓ(4 + mem Ⓓ[4 + (mem Ⓓ[4 + mem Ⓓ[48 + pxCurrentTCB gp mem]])]) /\
-        s R_A3 = Ⓓ(mem Ⓓ[4 + mem Ⓓ[48 + pxCurrentTCB gp mem]]) /\
-        s R_A4 = Ⓓ(mem Ⓓ[8 + mem Ⓓ[48 + pxCurrentTCB gp mem]]) /\
-        s R_A5 = Ⓓ(mem Ⓓ[12 + mem Ⓓ[48 + pxCurrentTCB gp mem]]) /\
+    | 0x80001418 => Some (exists mem gp, s V_MEM32 = Ⓜmem /\ 
+        s R_GP = Ⓓgp /\ s R_SP = Ⓓ(base_sp ⊖ 16) /\
+        s R_A1 = Ⓓ(mem Ⓓ[4 + mem Ⓓ[(gp ⊖ 920) ⊕ ((31 ⊖ (clz (uxTopReadyPriority gp mem) 32)) * 20)]]) /\
+        s R_A2 = Ⓓ(addr_pxReadyTasksLists gp ⊕ ((31 ⊖ (clz (uxTopReadyPriority gp mem) 32)) * 20)) /\
+        s R_A3 = Ⓓ(31 ⊖ clz (uxTopReadyPriority gp mem) 32) /\
+        s R_A4 = Ⓓ(addr_pxReadyTasksLists gp) /\
+        s R_A5 = Ⓓ((gp ⊖ 916) ⊕ (31 ⊖ clz (uxTopReadyPriority gp mem) 32) * 20) /\
         gp_sp_noverlap gp base_sp /\
         smem_well_formed gp /\
+        pxCurrentTCB_noverlap_static gp mem /\
+        pxCurrentTCB_noverlap_stackframe gp base_sp mem /\
+        mem_pxCurrentTCB_noverlap_stackframe gp base_sp mem /\
+        mem_pxCurrentTCB_noverlap_static gp mem /\
         (uxSchedulerSuspended gp mem =? 0) = true /\
-        (* cycle_count_of_trace t' = 17 + 2 * time_branch + 11 * time_mem) *)
         cycle_count_of_trace t' = 36 + clz (mem Ⓓ[ 4294965376 + gp ]) 32 + 2 * time_branch + 14 * time_mem)
     | 0x8000138c => Some (exists mem gp, s V_MEM32 = Ⓜmem /\ s R_GP = Ⓓgp /\ timing_postcondition t gp mem)
     | 0x8000144c => Some (
@@ -276,6 +331,12 @@ Now we can specialize assumption for pxcurrenttcb, uxschedulersuspended etc.
 Do we assume that these buffers don't overlap with stack frame?
 *)
 
+Theorem clz_le_w : forall n w,
+    clz n w <= w.
+Proof.
+    destruct n; intros; unfold clz; lia.
+Qed.
+
 Theorem vTaskSwitchContext_timing:
   forall s p t s' x' gp sp mem
          (ENTRY: startof t (x',s') = (Addr start_vTaskSwitchContext,s)) (* Define the entry point of the function *)
@@ -284,6 +345,10 @@ Theorem vTaskSwitchContext_timing:
          (SP : s R_SP = Ⓓsp)
          (MEM : s V_MEM32 = Ⓜmem)
          (GP_SP_FAR : gp_sp_noverlap gp sp)
+         (PCT_NOL_STATIC : pxCurrentTCB_noverlap_static gp mem)
+         (PCT_NOL_SFRAME : pxCurrentTCB_noverlap_stackframe gp sp mem)
+         (MEM_PCT_NOL_SFRAME : mem_pxCurrentTCB_noverlap_stackframe gp sp mem)
+         (MEM_PCT_NOL_STATIC : mem_pxCurrentTCB_noverlap_static gp mem)
          (SMEM_WELL_FORMED : smem_well_formed gp)
          (* (TCB_STACK_NO : ~ overlap 32 (pxCurrentTCB gp mem) 52 (sp ⊖ 16) 16) *)
          ,
@@ -318,17 +383,70 @@ Proof using.
     destruct_inv 32 PRE.
 
     (* 0x800015e4 *)
-    destruct PRE as [mem [gp [MEM [GP [SP [A4 [GP_SP_FAR [SMEM_WELL_FORMED Cycles]]]]]]]].
+    destruct PRE as [mem [gp [MEM [GP [SP [A4 [GP_SP_FAR [SMEM_WELL_FORMED 
+        [PCT_NOL_STATIC [PCT_NOL_SFRAME [MEM_PCT_NOL_SFRAME [MEM_PCT_NOL_STATIC 
+        Cycles]]]]]]]]]]]].
     step. step. step. step. step. step. step. step. step. step.
     do 2 eexists. repeat split. unfold msub. now psimpl.
         {
-            noverlap_prepare gp sp; memsolve mem gp sp.
-            all: admit. (* Down to pxCurrentTCB overlaps *)
+            noverlap_prepare gp sp.
+            rewrite <- getmem_mod_l with (a := 4294965400 + gp);
+            replace (4294965400 ⊕ gp) with (gp ⊖ 1896) by 
+                (unfold msub; psimpl; lia).
+            memsolve mem gp sp; 
+            try solve [ now (
+                apply PCT_NOL_STATIC ||
+                apply PCT_NOL_SFRAME
+            )].
+            all: apply noverlap_symmetry;
+                (apply noverlap_shrink with (sp ⊖ 16) 16;
+                    [ psimpl; lia | apply noverlap_symmetry]);
+                assumption.
         }
         {
-            noverlap_prepare gp sp; memsolve mem gp sp.
-            all: admit. (* Down to pxCurrentTCB overlaps *)
+            noverlap_prepare gp sp.
+            rewrite <- getmem_mod_l with (a := 4294965400 + gp);
+            replace (4294965400 ⊕ gp) with (gp ⊖ 1896) by 
+                (unfold msub; psimpl; lia).
+            memsolve mem gp sp;
+            try solve [ now (
+                apply PCT_NOL_STATIC ||
+                apply PCT_NOL_SFRAME ||
+                apply MEM_PCT_NOL_STATIC
+            )].
+            all: try solve [apply noverlap_symmetry;
+                (apply noverlap_shrink with (sp ⊖ 16) 16;
+                    [ psimpl; lia | apply noverlap_symmetry]);
+                assumption].
         } assumption. assumption.
+        {
+            unfold pxCurrentTCB_noverlap_static in *.
+            intros. noverlap_prepare gp sp. memsolve mem gp sp.
+            apply PCT_NOL_STATIC, H.
+        }
+        {
+            unfold pxCurrentTCB_noverlap_stackframe in *.
+            intros. noverlap_prepare gp sp. memsolve mem gp sp.
+            apply PCT_NOL_SFRAME.
+        }
+        {
+            unfold mem_pxCurrentTCB_noverlap_stackframe in *.
+            intros. noverlap_prepare gp sp. memsolve mem gp sp.
+                apply MEM_PCT_NOL_SFRAME.
+                now apply PCT_NOL_STATIC.
+                all: apply noverlap_symmetry, noverlap_shrink with (sp ⊖ 16) 16;
+                    [ psimpl; lia |
+                      apply noverlap_symmetry, PCT_NOL_SFRAME ].
+        }
+        {
+            unfold mem_pxCurrentTCB_noverlap_static in *.
+            intros. noverlap_prepare gp sp. memsolve mem gp sp.
+                now apply MEM_PCT_NOL_STATIC.
+                now apply PCT_NOL_STATIC.
+                all: apply noverlap_symmetry, noverlap_shrink with (sp ⊖ 16) 16;
+                    [ psimpl; lia |
+                      apply noverlap_symmetry, PCT_NOL_SFRAME ].
+        }
         { noverlap_prepare gp sp. memsolve mem gp sp. assumption. }
         hammer. rewrite A4, BC, Cycles. lia.
     step. step. handle_ex.
@@ -338,8 +456,9 @@ Proof using.
         hammer. rewrite A4, BC, Cycles. lia.
 
     (* 0x800013c8 *)
-    destruct PRE as [mem [gp [MEM [GP [SP [A5 [A2 [A4 
-        [GP_SP_FAR [SMEM_WELL_FORMED [BR0 Cycles]]]]]]]]]]].
+    destruct PRE as [mem [gp [MEM [GP [SP [A5 [A2 [A4 [GP_SP_FAR [SMEM_WELL_FORMED 
+        [PCT_NOL_STATIC [PCT_NOL_SFRAME [MEM_PCT_NOL_SFRAME [MEM_PCT_NOL_STATIC 
+        [BR0 Cycles]]]]]]]]]]]]]]].
     step.
         step. step. step. step. step. step. step. step. step. step.
         exact I. (* Infinite loop, stack overflow detected *)
@@ -348,8 +467,9 @@ Proof using.
         hammer. rewrite A2, A4, BC, Cycles. lia.
 
     (* 0x800013d0 *)
-    destruct PRE as [mem [gp [MEM [GP [A2 [A3 [A5 [GP_SP_FAR [SMEM_WELL_FORMED 
-        [NotSuspended [Br Cycles]]]]]]]]]]].
+    destruct PRE as [mem [gp [MEM [GP [SP [A2 [A3 [A5 [GP_SP_FAR [SMEM_WELL_FORMED 
+        [PCT_NOL_STATIC [PCT_NOL_SFRAME [MEM_PCT_NOL_SFRAME [MEM_PCT_NOL_STATIC 
+        [NotSuspended [Br Cycles]]]]]]]]]]]]]]]].
     step.
         step. step. step. step. step. step. step. step. step. step.
         exact I. (* Infinite loop, stack overflow detected *)
@@ -358,8 +478,9 @@ Proof using.
         hammer. rewrite A2, A3, Cycles, BC. lia.
 
     (* 0x800013d8 *)
-    destruct PRE as [mem [gp [MEM [GP [A3 [A4 [A5 [GP_SP_FAR [SMEM_WELL_FORMED 
-        [B1 [B2 [NotSuspended Cycles]]]]]]]]]]]].
+    destruct PRE as [mem [gp [MEM [GP [SP [A3 [A4 [A5 [GP_SP_FAR [SMEM_WELL_FORMED 
+        [PCT_NOL_STATIC [PCT_NOL_SFRAME [MEM_PCT_NOL_SFRAME [MEM_PCT_NOL_STATIC 
+        [B1 [B2 [NotSuspended Cycles]]]]]]]]]]]]]]]]].
     step.
         step. step. step. step. step. step. step. step. step. step.
         exact I. (* Infinite loop, stack overflow detected *)
@@ -369,15 +490,162 @@ Proof using.
         hammer. rewrite A3, A4, BC, Cycles. lia.
 
     (* 0x800013e0 *)
-    destruct PRE as [mem [gp [MEM [GP [A3 [A4 [A5 [GP_SP_FAR [SMEM_WELL_FORMED 
-        [B1 [B2 [B3 [NotSuspended Cycles]]]]]]]]]]]]].
+    destruct PRE as [mem [gp [MEM [GP [SP [A3 [A4 [A5 [GP_SP_FAR [SMEM_WELL_FORMED 
+        [PCT_NOL_STATIC [PCT_NOL_SFRAME [MEM_PCT_NOL_SFRAME [MEM_PCT_NOL_STATIC 
+        [B1 [B2 [B3 [NotSuspended Cycles]]]]]]]]]]]]]]]]]].
     step. step. step. step. step. step. step. step. step. step. step.
     step. step. step. step.
         handle_ex. repeat split.
-        admit. admit. admit. admit. (* CLZ noverlap *)
         {
-            noverlap_prepare gp sp; memsolve mem gp sp. assumption.
-            admit. (* CLZ noverlap *)
+            noverlap_prepare gp sp.
+            rewrite <- getmem_mod_l with (a := 4294965376 + gp);
+            replace (4294965376 ⊕ gp) with (gp ⊖ 1920) by 
+                (unfold msub; psimpl; lia).
+            rewrite <- getmem_mod_l with (a := 4294966376 + gp + 
+                (31 ⊖ clz (mem Ⓓ[ gp ⊖ 1920 ]) 32) * 20).
+            replace (mem Ⓓ[ 4294966376 + gp ⊕ (31 ⊖ clz (mem Ⓓ[ gp ⊖ 1920 ]) 32) * 20 ])
+            with (mem Ⓓ[ gp ⊖ 920 ⊕ (31 ⊖ clz (mem Ⓓ[ gp ⊖ 1920 ]) 32) * 20 ]); cycle 7.
+            unfold msub at 1. now psimpl. unfold uxTopReadyPriority.
+            memsolve mem gp sp; unfold msub at 1; psimpl.
+            apply sep_noverlap; left; psimpl;
+                pose proof (clz_le_w (mem Ⓓ[ gp ⊖ 1920 ]) 32);
+                remember (clz (mem Ⓓ[ gp ⊖ 1920 ]) 32) as n; clear Heqn;
+                do 33 (destruct n as [| n _] using N.peano_ind;
+                    [cbn [N.succ Pos.succ]; psimpl; lia|
+                    replace (N.succ n) with (1 + n) in H by lia; psimpl in H]);
+                lia.
+            admit. (* actual overlaps *)
+            apply sep_noverlap; left; psimpl;
+                pose proof (clz_le_w (mem Ⓓ[ gp ⊖ 1920 ]) 32);
+                remember (clz (mem Ⓓ[ gp ⊖ 1920 ]) 32) as n; clear Heqn;
+                do 33 (destruct n as [| n _] using N.peano_ind;
+                    [cbn [N.succ Pos.succ]; psimpl; lia|
+                    replace (N.succ n) with (1 + n) in H by lia; psimpl in H]);
+                lia.
+            admit. (* Don't even know what's going on here *)
+            apply sep_noverlap; left; psimpl;
+                pose proof (clz_le_w (mem Ⓓ[ gp ⊖ 1920 ]) 32);
+                remember (clz (mem Ⓓ[ gp ⊖ 1920 ]) 32) as n; clear Heqn;
+                do 33 (destruct n as [| n _] using N.peano_ind;
+                    [cbn [N.succ Pos.succ]; psimpl; lia|
+                    replace (N.succ n) with (1 + n) in H by lia; psimpl in H]);
+                lia.
+            admit. (* actual overlaps *)
+            apply sep_noverlap; left; psimpl;
+                pose proof (clz_le_w (mem Ⓓ[ gp ⊖ 1920 ]) 32);
+                remember (clz (mem Ⓓ[ gp ⊖ 1920 ]) 32) as n; clear Heqn;
+                do 33 (destruct n as [| n _] using N.peano_ind;
+                    [cbn [N.succ Pos.succ]; psimpl; lia|
+                    replace (N.succ n) with (1 + n) in H by lia; psimpl in H]);
+                lia.
+        }
+        {
+            unfold addr_pxReadyTasksLists, uxTopReadyPriority.
+            noverlap_prepare gp sp; memsolve mem gp sp. f_equal.
+                unfold msub; psimpl.
+                replace (2 ^ 32 - 1920 mod 2 ^ 32) with 4294965376 by reflexivity.
+                now rewrite getmem_mod_l, (N.add_comm gp).
+            unfold msub at 1; psimpl.
+            apply sep_noverlap; left; psimpl;
+                pose proof (clz_le_w (mem Ⓓ[ 4294965376 + gp ]) 32);
+                remember (clz (mem Ⓓ[ 4294965376 + gp ]) 32) as n; clear Heqn;
+                do 33 (destruct n as [| n _] using N.peano_ind;
+                    [cbn [N.succ Pos.succ]; psimpl; lia|
+                    replace (N.succ n) with (1 + n) in H by lia; psimpl in H]);
+                lia.
+        }
+        {
+            unfold uxTopReadyPriority.
+            noverlap_prepare gp sp; memsolve mem gp sp.
+                unfold msub at 3. simpl (_ - _ mod _).
+                now rewrite getmem_mod_l, (N.add_comm 4294965376).
+            apply sep_noverlap; left; psimpl;
+                pose proof (clz_le_w (mem Ⓓ[ 4294965376 + gp ]) 32);
+                remember (clz (mem Ⓓ[ 4294965376 + gp ]) 32) as n; clear Heqn;
+                do 33 (destruct n as [| n _] using N.peano_ind;
+                    [cbn [N.succ Pos.succ]; psimpl; lia|
+                    replace (N.succ n) with (1 + n) in H by lia; psimpl in H]);
+                lia.
+        }
+        now unfold addr_pxReadyTasksLists, msub; psimpl.
+        {
+            unfold uxTopReadyPriority.
+            noverlap_prepare gp sp; memsolve mem gp sp. f_equal.
+                unfold msub at 2 4. simpl (_ - _ mod _).
+                rewrite N.add_comm, N.add_assoc.
+                rewrite (N.add_comm _ gp), getmem_mod_l. now psimpl.
+            apply sep_noverlap; left; psimpl;
+                pose proof (clz_le_w (mem Ⓓ[ 4294965376 + gp ]) 32);
+                remember (clz (mem Ⓓ[ 4294965376 + gp ]) 32) as n; clear Heqn;
+                do 33 (destruct n as [| n _] using N.peano_ind;
+                    [cbn [N.succ Pos.succ]; psimpl; lia|
+                    replace (N.succ n) with (1 + n) in H by lia; psimpl in H]);
+                lia.
+        }
+        {
+            unfold pxCurrentTCB_noverlap_static. intros.
+            noverlap_prepare gp sp; memsolve mem gp sp.
+            now apply PCT_NOL_STATIC.
+            unfold msub at 1. simpl (_ - _ mod _).
+            apply sep_noverlap; left; psimpl;
+                pose proof (clz_le_w (mem Ⓓ[ 4294965376 + gp ]) 32);
+                remember (clz (mem Ⓓ[ 4294965376 + gp ]) 32) as n; clear Heqn;
+                do 33 (destruct n as [| n _] using N.peano_ind;
+                    [cbn [N.succ Pos.succ]; psimpl; lia|
+                    replace (N.succ n) with (1 + n) in H by lia; psimpl in H]);
+                lia.
+        }
+        {
+            unfold pxCurrentTCB_noverlap_stackframe. intros.
+            noverlap_prepare gp sp; memsolve mem gp sp.
+            now apply PCT_NOL_SFRAME.
+            unfold msub at 1. simpl (_ - _ mod _).
+            apply sep_noverlap; left; psimpl;
+                pose proof (clz_le_w (mem Ⓓ[ 4294965376 + gp ]) 32);
+                remember (clz (mem Ⓓ[ 4294965376 + gp ]) 32) as n; clear Heqn;
+                do 33 (destruct n as [| n _] using N.peano_ind;
+                    [cbn [N.succ Pos.succ]; psimpl; lia|
+                    replace (N.succ n) with (1 + n) in H by lia; psimpl in H]);
+                lia.
+        }
+        {
+            unfold mem_pxCurrentTCB_noverlap_stackframe.
+            noverlap_prepare gp sp; memsolve mem gp sp.
+            now apply MEM_PCT_NOL_SFRAME.
+            all: unfold msub at 1; simpl (_ - _ mod _);
+            try (apply sep_noverlap; left; psimpl;
+                pose proof (clz_le_w (mem Ⓓ[ 4294965376 + gp ]) 32);
+                remember (clz (mem Ⓓ[ 4294965376 + gp ]) 32) as n; clear Heqn;
+                do 33 (destruct n as [| n _] using N.peano_ind;
+                    [cbn [N.succ Pos.succ]; psimpl; lia|
+                    replace (N.succ n) with (1 + n) in H by lia; psimpl in H]);
+                lia).
+            admit. (* Deeper CLZ noverlap *)
+        }
+        {
+            unfold mem_pxCurrentTCB_noverlap_static. intros.
+            noverlap_prepare gp sp; memsolve mem gp sp.
+            now apply MEM_PCT_NOL_STATIC.
+            all: unfold msub at 1; simpl (_ - _ mod _);
+            try (apply sep_noverlap; left; psimpl;
+                pose proof (clz_le_w (mem Ⓓ[ 4294965376 + gp ]) 32);
+                remember (clz (mem Ⓓ[ 4294965376 + gp ]) 32) as n; clear Heqn;
+                do 33 (destruct n as [| n _] using N.peano_ind;
+                    [cbn [N.succ Pos.succ]; psimpl; lia|
+                    replace (N.succ n) with (1 + n) in H by lia; psimpl in H]);
+                lia).
+            admit. (* Deeper CLZ noverlap *)
+        }
+        {
+            noverlap_prepare gp sp; memsolve mem gp sp.
+            assumption.
+            apply sep_noverlap; left; psimpl;
+                pose proof (clz_le_w (mem Ⓓ[ 4294965376 + gp ]) 32);
+                remember (clz (mem Ⓓ[ 4294965376 + gp ]) 32) as n; clear Heqn;
+                do 33 (destruct n as [| n _] using N.peano_ind;
+                    [cbn [N.succ Pos.succ]; psimpl; lia|
+                    replace (N.succ n) with (1 + n) in H by lia; psimpl in H]);
+                lia.
         }
         hammer. rewrite A4, A5, BC, Cycles. psimpl.
         (* Can't infer placeholder? *)
@@ -389,22 +657,15 @@ Proof using.
         lia.
         {
             noverlap_prepare gp sp. memsolve mem gp sp.
-            apply sep_noverlap; left; psimpl.
-            - clear. induction (31 ⊖ (clz _ _)) using N.peano_ind; psimpl.
-                lia. replace (N.succ n) with (1 + n) by lia.
-                rewrite N.mul_add_distr_r. psimpl.
-                etransitivity. eassumption. admit.
-            - clear. induction (31 ⊖ (clz _ _)) using N.peano_ind; psimpl. lia.
-                unfold msub. replace (N.succ n) with (1 + n) by lia.
-                rewrite N.mul_add_distr_r. psimpl.
-                admit.
+            apply sep_noverlap; left; psimpl; admit. (* CLZ noverlap *)
         }
     (* Inside vApplicationStackOverflowHook *)
     step. step. step. step. step. step. step. step. step. step. exact I.
 
     (* 0x8000142c *)
-    destruct PRE as [mem [gp [MEM [GP [A1 [A3 [A4 [A5 [GP_SP_FAR [SMEM_WELL_FORMED 
-        [NotSuspended Cycles]]]]]]]]]]].
+    destruct PRE as [mem [gp [MEM [GP [SP [A1 [A2 [A3 [A4 [A5 [GP_SP_FAR 
+        [SMEM_WELL_FORMED [PCT_NOL_STATIC [PCT_NOL_SFRAME [MEM_PCT_NOL_SFRAME
+        [MEM_PCT_NOL_STATIC [NotSuspended Cycles]]]]]]]]]]]]]]]]].
     step. step. step. step. step. step. step. step. step. step. step.
         handle_ex.
         {
@@ -448,19 +709,27 @@ Proof using.
         | _ => idtac end.
         cbn [negb].
         replace (clz
-        ((mem [Ⓓ4 + n := mem Ⓓ[ 12 + n ] ] [Ⓓ4294965400 + gp
-          := (mem [Ⓓ4 + n := mem Ⓓ[ 12 + n ] ])
-             Ⓓ[ 12 +
-                (mem [Ⓓ4 + n := mem Ⓓ[ 12 + n ] ])
+        ((mem [Ⓓ4294966376 + gp + (31 ⊖ clz (mem Ⓓ[ gp ⊖ 1920 ]) 32) * 20
+            := mem Ⓓ[ 4294966384 + gp + (31 ⊖ clz (mem Ⓓ[ gp ⊖ 1920 ]) 32) * 20 ] ]
+            [Ⓓ4294965400 + gp
+            := (mem [Ⓓ4294966376 + gp + (31 ⊖ clz (mem Ⓓ[ gp ⊖ 1920 ]) 32) * 20
+                := mem Ⓓ[ 4294966384 + gp + (31 ⊖ clz (mem Ⓓ[ gp ⊖ 1920 ]) 32) * 20
+                ] ])
+            Ⓓ[ 12 +
+                (mem [Ⓓ4294966376 + gp + (31 ⊖ clz (mem Ⓓ[ gp ⊖ 1920 ]) 32) * 20
+                := mem
+                    Ⓓ[ 4294966384 + gp + (31 ⊖ clz (mem Ⓓ[ gp ⊖ 1920 ]) 32) * 20 ]
+                ])
                 Ⓓ[ 4 + mem Ⓓ[ 8 + mem Ⓓ[ 48 + pxCurrentTCB gp mem ] ] +
-                   mem Ⓓ[ 4 + mem Ⓓ[ 48 + pxCurrentTCB gp mem ] ] * 20 ] ] ]) Ⓓ[ 
-         4294965376 + gp ]) 32) with (clz (mem Ⓓ[ 4294965376 + gp ]) 32).
+                    mem Ⓓ[ 4 + mem Ⓓ[ 48 + pxCurrentTCB gp mem ] ] * 20 ] ] ])
+        Ⓓ[ 4294965376 + gp ]) 32) with (clz (mem Ⓓ[ 4294965376 + gp ]) 32).
         lia.
-        { admit. (* pxCurrentTCB noverlaps, also some SP stuff. Need to bind to current SP
-            and update gp_sp_noverlap so that it takes into account the difference to SP over time *) }
+        { f_equal. noverlap_prepare gp sp. memsolve mem gp sp.
+            admit. (* CLZ noverlap *)
+        }
         { admit. (* More actual overlapping stuff *) }
         { noverlap_prepare gp n0. memsolve mem gp n0. now rewrite NotSuspended.
-          admit. (* Need to pass in gp_sp_noverlap *) }
+          admit. (* CLZ noverlap *) }
 
     step. exact I.
 Admitted.
